intermediate2/Zeta.Intermediate.Blum.fsti
@@ -1,0 +1,47 @@
+module Zeta.Intermediate.Blum
+
+open Zeta.Time
+open Zeta.Generic.Interleave
+open Zeta.Generic.Blum
+open Zeta.High.Interleave
+open Zeta.Intermediate.Interleave
+
+val lemma_spec_rel_implies_same_add_elem (#vcfg:_)
+  (il: verifiable_log vcfg {spec_rel il})
+  (i: seq_index il {is_blum_add il i})
+  : Lemma (ensures (let ilk = to_logk il in
+                    is_blum_add ilk i /\
+                    blum_add_elem il i = blum_add_elem ilk i))
+          [SMTPat (blum_add_elem il i)]
+
+val lemma_spec_rel_implies_same_evict_elem (#vcfg:_)
+  (il: verifiable_log vcfg {spec_rel il})
+  (i: seq_index il {is_blum_evict il i})
+  : Lemma (ensures (let ilk = to_logk il in
+                    is_blum_evict ilk i /\
+                    blum_evict_elem il i = blum_evict_elem ilk i))
+          [SMTPat (blum_evict_elem il i)]
+
+val lemma_spec_rel_implies_same_add_seq (#vcfg:_) (ep: epoch) (il: verifiable_log vcfg)
+  : Lemma (requires (spec_rel il))
+          (ensures (let ilk = to_logk il in
+                    add_seq ep il == add_seq ep ilk))
+          [SMTPat (add_seq ep il)]
+
+val lemma_spec_rel_implies_same_evict_seq (#vcfg:_) (ep: epoch) (il: verifiable_log vcfg)
+  : Lemma (requires (spec_rel il))
+          (ensures (let ilk = to_logk il in
+                    evict_seq ep il == evict_seq ep ilk))
+          [SMTPat (evict_seq ep il)]
+
+val lemma_spec_rel_implies_same_add_set (#vcfg:_) (ep: epoch) (il: verifiable_log vcfg)
+  : Lemma (requires (spec_rel il))
+          (ensures (let ilk = to_logk il in
+                    add_set ep il == add_set ep ilk))
+          [SMTPat (add_set ep il)]
+
+val lemma_spec_rel_implies_same_evict_set (#vcfg:_) (ep: epoch) (il: verifiable_log vcfg)
+  : Lemma (requires (spec_rel il))
+          (ensures (let ilk = to_logk il in
+                    evict_set ep il == evict_set ep ilk))
+          [SMTPat (evict_set ep il)]
